more progress on buf/specs.v

src/program_proof/buf/specs.v
@@ -6,7 +6,8 @@ From Perennial.program_proof Require Import proof_prelude.
 From Perennial.Helpers Require Import GenHeap.
 From Perennial.goose_lang.lib Require Import struct.
 
-From Goose.github_com.mit_pdos.goose_nfsd Require Import addr buf.
+From Goose.github_com.mit_pdos.goose_nfsd Require Import buf.
+From Perennial.program_proof.addr Require Import specs.
 
 Section heap.
 Context `{!heapG Σ}.
@@ -15,6 +16,52 @@ Context `{!lockG Σ}.
 Implicit Types s : Slice.t.
 Implicit Types (stk:stuckness) (E: coPset).
 
+Definition inode_bytes := Z.to_nat 128.
+Definition inode_buf := vec u8 inode_bytes.
+Definition inode_to_vals {ext: ext_op} (i:inode_buf) : list val :=
+  fmap b2val (vec_to_list i).
+
+Inductive bufDataT :=
+| bufBit (b : bool)
+| bufInode (i : inode_buf)
+| bufBlock (b : Block)
+.
+
+Record buf := {
+  bufData : bufDataT;
+  bufDirty : bool;
+}.
+
+Definition get_bit (b0 : u8) (off : u64) : bool.
+Admitted.
+
+Definition is_bufObject (bufptr : loc) (a : addr) (o : buf) : iProp Σ :=
+  ∃ (data : Slice.t) (sz : u64),
+    bufptr ↦[Buf.S :: "Addr"] (addr2val a) ∗
+    bufptr ↦[Buf.S :: "Sz"] #sz ∗
+    bufptr ↦[Buf.S :: "Data"] (slice_val data) ∗
+    bufptr ↦[Buf.S :: "dirty"] #o.(bufDirty) ∗
+    ⌜ valid_addr a ⌝ ∗
+    match o.(bufData) with
+    | bufBit b => ∃ (b0 : u8), is_slice data u8T 1%Qp (#b0 :: nil) ∗
+      ⌜ get_bit b0 (word.modu a.(addrOff) 8) ⌝ ∗
+      ⌜ sz = 1 ⌝
+    | bufInode i => is_slice data u8T 1%Qp (inode_to_vals i) ∗
+      ⌜ sz = (inode_bytes * 8)%nat ⌝
+    | bufBlock b => is_slice data u8T 1%Qp (Block_to_vals b) ∗
+      ⌜ sz = (block_bytes * 8)%nat ⌝
+    end.
+
+Definition is_bufmap (bufmap : loc) (bm : gmap addr buf) : iProp Σ :=
+  ∃ (mptr : loc) (m : gmap u64 val) (am : gmap addr val) def,
+    bufmap ↦[BufMap.S :: "addrs"] #mptr ∗
+    is_map mptr (m, def) ∗
+    ⌜ flatid_addr_map m am ⌝ ∗
+    [∗ map] a ↦ bufptr; buf ∈ am; bm,
+      ∃ (bufloc : loc),
+        ⌜ bufptr = #bufloc ⌝ ∗
+        is_bufObject bufloc a buf.
+
 Theorem wp_MkBufMap :
   {{{
     emp
@@ -22,7 +69,7 @@ Theorem wp_MkBufMap :
     MkBufMap #()
   {{{
     (l : loc), RET #l;
-    emp
+    is_bufmap l ∅
   }}}.
 Proof.
   iIntros (Φ) "Hemp HΦ".
@@ -34,8 +81,15 @@ Opaque zero_val. (* XXX can we avoid this? *)
   wp_apply wp_allocStruct; eauto.
   iIntros (bufmap) "Hbufmap".
 
+  iDestruct (struct_fields_split with "Hbufmap") as "[Hbufmap _]".
+
   wp_pures.
   iApply "HΦ".
+  iExists _, _, _, _.
+
+  iFrame.
+  iSplitR; first (iPureIntro; apply flatid_addr_empty).
+  iApply big_sepM2_empty.
   done.
 Qed.
 
